modification on directed actions

theories/DirectedErasure.v
@@ -5,13 +5,14 @@ From LogRel.AutoSubst Require Import core unscoped Ast Extra.
 From LogRel Require Import Utils BasicAst Notations Context DeclarativeTyping DeclarativeInstance Weakening GenericTyping.
 
 From LogRel Require Import DirectedDirections.
-From LogRel Require DirectedDeclarativeTyping DirectedContext.
+From LogRel Require Import DirectedDeclarativeTyping DirectedContext.
 
 
+Import Notations.
 Import DeclarativeTypingData.
 Import DeclarativeTypingProperties.
 
-Fixpoint erase_dir (ctx: DirectedContext.context) : context :=
+Fixpoint erase_dir (ctx: DirectedContext.context) : Context.context :=
   match ctx with
   | nil => nil
   | cons {| DirectedContext.ty := T |} l => cons T (erase_dir l)
@@ -20,22 +21,21 @@ Fixpoint erase_dir (ctx: DirectedContext.context) : context :=
 
 Lemma in_ctx_erased {Θ n decl} :
   DirectedContext.in_ctx Θ n decl ->
-  in_ctx (erase_dir Θ) n (DirectedContext.ty decl).
+  Context.in_ctx (erase_dir Θ) n (DirectedContext.ty decl).
 Proof.
   induction 1; now constructor.
 Qed.
 
 Lemma typing_erased :
-  (forall Θ : DirectedContext.context,
-      DirectedDeclarativeTyping.WfContextDecl Θ -> [ |- erase_dir Θ ])
-    × (forall (Θ : DirectedContext.context) (d: direction) (A : term),
-        DirectedDeclarativeTyping.WfTypeDecl Θ d A -> [ erase_dir Θ |- A ])
-    × (forall (Θ : DirectedContext.context) (dt: direction) (A: term) (dA: direction) (t : term),
-        DirectedDeclarativeTyping.TypingDecl Θ dt A dA t -> [ erase_dir Θ |- t : A ])
-    × (forall (Θ : DirectedContext.context) (d: direction) (A B : term),
-        DirectedDeclarativeTyping.ConvTypeDecl Θ d A B -> [ erase_dir Θ |- A ≅ B ])
-    × (forall (Θ : DirectedContext.context) (dt: direction) (A : term) (dA: direction) (t u : term),
-        DirectedDeclarativeTyping.ConvTermDecl Θ dt A dA t u -> [ erase_dir Θ |- t ≅ u : A ]).
+  (forall Θ, [ |-( ) Θ ] -> [ |- erase_dir Θ ])
+    × (forall Θ d A,
+        [ Θ |-( d ) A] -> [ erase_dir Θ |- A ])
+    × (forall Θ dt A dA t,
+        [ Θ |-( dt ) t : A @ dA ] -> [ erase_dir Θ |- t : A ])
+    × (forall Θ d A B,
+        [ Θ |-( d ) A ≅ B ] -> [ erase_dir Θ |- A ≅ B ])
+    × (forall Θ dt A dA t u,
+        [ Θ |-( dt ) t ≅ u : A @ dA ] -> [ erase_dir Θ |- t ≅ u : A ]).
 Proof.
   eapply DirectedDeclarativeTyping.WfDeclInduction.
   all: try now econstructor.
