theories/DirectedPartialTranslation.v
@@ -3,7 +3,7 @@ From Coq Require Import ssreflect.
 From Equations Require Import Equations.
 From smpl Require Import Smpl.
 From LogRel.AutoSubst Require Import core unscoped Ast Extra.
-From LogRel Require Import Utils BasicAst Notations Context DeclarativeTyping Weakening GenericTyping.
+From LogRel Require Import Utils BasicAst Notations Context NormalForms DeclarativeTyping Weakening GenericTyping.
 
 From LogRel Require Import DirectedDirections DirectedErasure.
 From LogRel Require DirectedDeclarativeTyping DirectedContext.
@@ -15,18 +15,14 @@ Set Universe Polymorphism.
 Import IndexedDefinitions.
 Import StdInstance.
 
-
-Definition witType (d: direction) : Type :=
-  match d with
-  | Fun | Cofun => term
-  | Discr => unit
-  end.
-
-Definition witList := list (∑ (d: direction), witType d).
-
-Equations tsl_fun (γ : witList) : (direction × term) ⇀ term :=
-  tsl_fun γ (d, (tSort s)) := ret (tLambda (tSort s) (tRel 0)) ;
-  tsl_fun γ _ := undefined.
-
-
+(* NOTE: no need to handle lambda, because we only look at types in whnf *)
+Equations type_action (γ : list (option term)) : term ⇀ term :=
+  type_action γ (tSort s) := ret (tLambda (tSort s) (tRel 0)) ;
+  type_action γ (tProd A B) := tB ← rec B ;; ret (tLambda A tB) ;
+  type_action γ (tRel n) := match List.nth n γ None with
+                        | Some t => ret t
+                        | None => undefined
+                        end ;
+  type_action γ (tApp f a) := tf ← rec f ;; ret (tApp tf a) ;
+  type_action γ _ := undefined.
 
